Add lean-format flake target.

SkLean/Dsl.lean
@@ -17,7 +17,7 @@ def to_sk_expr (names : List String) : NamedSkExpr → SkExpr
   | .prp => .prp
   | .ty n => .ty n
   | .call lhs rhs => .call (to_sk_expr names lhs) (to_sk_expr names rhs)
-  | .var name => .var $ ⟨(names.findIdx? (. = name)).getD 0⟩
+  | .var name => .var $ ⟨Nat.succ <| (names.findIdx? (. = name)).getD 0⟩
   | .fall name bind_ty body => .fall
       (to_sk_expr (name :: names) bind_ty)
       (to_sk_expr (name :: names) body)
@@ -33,6 +33,7 @@ syntax "∀"  ident ":" skexpr "," skexpr  : skexpr
 syntax "(" skexpr skexpr ")"                       : skexpr
 syntax "(" skexpr ")"                              : skexpr
 syntax ident                                       : skexpr
+syntax skexpr "→" skexpr                           : skexpr
 
 syntax " ⟪ " skexpr " ⟫ " : term
 
@@ -43,6 +44,7 @@ macro_rules
   | `(⟪ Prop ⟫)           => `(NamedSkExpr.prp)
   | `(⟪ Type $n:num ⟫)    => `(NamedSkExpr.ty $n)
   | `(⟪ $var:ident ⟫)       => `(NamedSkExpr.var $(Lean.quote var.getId.toString))
+  | `(⟪ $e₁:skexpr → $e₂:skexpr ⟫) => `(⟪ ∀ x : $e₁, $e₂ ⟫)
   | `(⟪ ∀ $var:ident : $e_ty:skexpr , $body:skexpr ⟫) =>
     `(NamedSkExpr.fall $(Lean.quote var.getId.toString) ⟪ $e_ty ⟫ ⟪ $body ⟫)
   | `(⟪ ($e₁:skexpr $e₂:skexpr )⟫) => `(NamedSkExpr.call ⟪ $e₁ ⟫ ⟪ $e₂ ⟫)
@@ -56,3 +58,4 @@ macro_rules
 #eval SK[S]
 #eval SK[∀ x : Prop, (∀ y : x, Prop)]
 #eval SK[∀ α : α, (∀ β : β, (∀ x : α, (∀ y : β, α)))]
+#eval SK[Prop → Prop]
