SkLean/Sk.lean
@@ -1,27 +1,15 @@
 import SkLean.Ast
+import SkLean.Dsl
+import Mathlib.Tactic
 
 open SkExpr
-open SkType
 
-structure Ctx where
-  binder_tys : BindId → 
+abbrev Ctx := List SkExpr
 
-def substitute (n : BindId) (with_expr : SkType): SkType → SkType
-  | fall bind_ty body =>
-    fall (substitute n.succ with_expr bind_ty) (substitute n.succ with_expr body)
-  | var n' => if n == n' then with_expr else var $ n - 1
-  | ty n => ty n
+abbrev ty_k := SK[∀ α : Type 0, ∀ β : Type 0, α → β → α]
+abbrev ty_s := SK[∀ α : Type 0, ∀ β : Type 0, ∀ γ : Type 0, (α → β → γ) → (α → β) → α → γ]
 
-infixr:65 " ~> " => fall
-
-abbrev ty_k := (var ⟨1⟩) ~> (SkExpr.var 1) ~> (SkExpr.var 3) ~> (SkExpr.var 3) ~> (SkExpr.var 4)
-
---             α                 β                 γ               x : α → β → γ                                            y : α → β                             z : α             γ
-abbrev ty_s := (SkExpr.var 1) ~> (SkExpr.var 1) ~> (SkExpr.var 1) ~> ((SkExpr.var 4) ~> (SkExpr.var 4) ~> (SkExpr.var 4)) ~> ((SkExpr.var 5) ~> (SkExpr.var 4)) ~> (SkExpr.var 6) ~> (SkExpr.var 4)
-
-def specialize_ty_k (α β : SkExpr) := α ~> β ~> α
-def specialize_ty_s (α β γ : SkExpr) := (α ~> β ~> γ) ~> (α ~> β) ~> α ~> γ
-
+#eval SK[∀ α : Type 0, ∀ β : Type 0, α → β → α]
 
 inductive beta_eq : SkExpr → SkExpr → Prop
   | trivial e₁ e₂    : e₁ = e₂ → beta_eq e₁ e₂
@@ -31,18 +19,16 @@ inductive beta_eq : SkExpr → SkExpr → Prop
 
 inductive valid_judgement : Ctx → SkExpr → SkExpr → Prop
   | k ctx e t (h_is_k : match e with | SkExpr.k => true | _ => false) :
-    -- K α : ∀ β.∀ (x : α).∀ (y : β).α
     t = ty_k → valid_judgement ctx e t
   | s ctx e t (h_is_s : match e with | SkExpr.s => true | _ => false) :
-    -- ∀ α β γ (x : α → β → γ) (y : α → β) (z : α), γ
     t = ty_s → valid_judgement ctx e t
   | call ctx e t (lhs : SkExpr) (rhs : SkExpr) (t_lhs : SkExpr) (t_rhs : SkExpr) (h_is_call : match e with | call lhs' rhs' => lhs' = lhs ∧ rhs' = rhs | _ => false) :
-    valid_judgement ctx lhs t_lhs → valid_judgement ctx rhs t_rhs → t = body (substitute 0 rhs t_lhs) → valid_judgement ctx e t
+    valid_judgement ctx lhs t_lhs → valid_judgement ctx rhs t_rhs → t = (t_lhs.substitute ⟨0⟩ rhs).body → valid_judgement ctx e t
   | fall ctx e t bind_ty body t_body (h_is_fall : match e with | fall _ _ => true | _ => false) :
     valid_judgement (bind_ty :: ctx) body t_body →
     e = fall bind_ty body →
     t = t_body → valid_judgement ctx e t
-  | obvious ctx e t : (match e with | ty n => t = ty n.succ | prp => t = ty 0 | var (n + 1) => ctx[n]? = some t | _ => false) → valid_judgement ctx e t
+  | obvious ctx e t : (match e with | ty n => t = ty n.succ | prp => t = ty 0 | var ⟨n + 1⟩ => ctx[n]? = some t | _ => false) → valid_judgement ctx e t
   | beta_eq ctx e e₂ t : beta_eq e e₂ → valid_judgement ctx e₂ t → valid_judgement ctx e t
 
 inductive sn : SkExpr → Prop
@@ -50,16 +36,25 @@ inductive sn : SkExpr → Prop
   | hard    e : (sn ∘ eval_once) e → sn e
 
 inductive in_r : Ctx → SkExpr → SkExpr → Prop
-  -- K α β is in r if all of its one-step reduxes are in R
-  | k ctx t e α β (h_t : t = (specialize_ty_k α β)) : ∀ arg₁ arg₂,
-    valid_judgement ctx t e →
+  | k ctx e t α β (h_t : t = SK[α → β → α]) : ∀ arg₁ arg₂,
+    valid_judgement ctx e t →
     in_r ctx α arg₁ →
     in_r ctx (eval_once (call (call (call (call k α) β) arg₁) arg₂)) α →
-    in_r ctx t e
-  | s ctx t e α β γ (h_t : t = (specialize_ty_s α β γ)) : ∀ arg₁ arg₂ arg₃, sorry → in_r ctx e t
-  | obvious ctx t e (h_is_obv : match e with | ty _ => true | fall _ _ => true | _ => false) : valid_judgement ctx e t → in_r ctx t e
+    in_r ctx e t
+  | s ctx e t (α : SkExpr) (β : SkExpr) (γ : SkExpr) (h_t : t = SK[(α → β → γ) → (α → β) → α → γ]) : ∀ arg₁ arg₂ arg₃, sorry → in_r ctx e t
+  | obvious ctx e t (h_is_obv : match e with | ty _ => true | fall _ _ => true | _ => false) : valid_judgement ctx e t → in_r ctx e t
 
-lemma all_in_r_sn (ctx : Ctx) : ∀ e t, valid_judgement ctx e t → in_r ctx t e → sn e := sorry
+lemma all_k_arg_judgement_holds (ctx : Ctx) : ∀ α, valid_judgement ctx α SK[Type 0] → valid_judgement ctx SK[(K α)] SK[∀ β : Type 0, α → β → α] := by
+  intro α h_α
+  repeat unfold NamedSkExpr.to_sk_expr at *
+  simp
+  apply valid_judgement.call ctx (k.call (var ⟨1⟩)) ((ty 0).fall ((var { toNat := 1 }).fall ((var { toNat := 3 }).fall (var { toNat := 1 }))))
+  sorry
+
+lemma all_k_args_judgement_holds (ctx : Ctx) : ∀ α (β : SkExpr) arg₁ (arg₂ : SkExpr), valid_judgement ctx arg₁ α → valid_judgement ctx SK[((((K α) β) arg₁) arg₂)] α := by
+  intro α β arg₁ arg₂ h_t_arg₁
+  
+  sorry
 
 example : eval_once (call (call k k) k) = k := by
   unfold eval_once
@@ -68,127 +63,3 @@ example : eval_once (call (call k k) k) = k := by
 example : (eval_once ∘ eval_once) (call (call (call s k) k) k) = k := by
   unfold eval_once
   simp
-
--- K α : ∀ β.∀ (x : α).∀ (y : β).α
-example : valid_judgement ctx (call k (ty 1)) (fall (var 1) (fall (ty 1) (fall (var 3) (ty 1)))) := by
-  apply (valid_judgement.call ctx
-    -- e
-    (call k (ty 1))
-    -- t
-    (fall (var 1) (fall (ty 1) (fall (var 3) (ty 1))))
-    -- lhs
-    k
-    -- rhs
-    (ty 1)
-    -- t_lhs
-    (fall (SkExpr.var 1) (
-          fall (SkExpr.var 1) (fall (SkExpr.var 3) (fall (SkExpr.var 3) (SkExpr.var 4)))))
-    -- t_rhs
-    (ty 2)
-    (by simp)
-  )
-  simp [valid_judgement.k]
-  simp [valid_judgement.obvious]
-  unfold substitute
-  simp
-  repeat unfold substitute
-  simp
-  unfold body
-  simp
-
--- S α : ∀ β γ (x : α → β → γ) (y : α → ̱̱β) (z : α).γ
-
--- K α β : ∀ (x : α).∀ (y : β).α
-example : valid_judgement ctx (call (call k (ty 1)) (ty 2)) (fall (ty 1) (fall (ty 2) (ty 1))) := by
-  apply (valid_judgement.call ctx
-    -- e
-    (call (call k (ty 1)) (ty 2))
-    -- t
-    (fall (ty 1) (fall (ty 2) (ty 1)))
-    -- lhs
-    (call k (ty 1))
-    -- rhs
-    (ty 2)
-    -- t_lhs
-    (fall (var 1) (fall (ty 1) (fall (var 3) (ty 1))))
-    -- t_rhs
-    (ty 3)
-    (by simp)
-  )
-  apply (valid_judgement.call ctx
-    (k.call (ty 1))
-    ((var 1).fall ((ty 1).fall ((var 3).fall (ty 1))))
-    k
-    (ty 1)
-    (fall (SkExpr.var 1) (
-          fall (SkExpr.var 1) (fall (SkExpr.var 3) (fall (SkExpr.var 3) (SkExpr.var 4)))))
-    (ty 2)
-    (by simp)
-  )
-  simp [valid_judgement.k]
-  simp [valid_judgement.obvious]
-  repeat unfold substitute
-  unfold body
-  simp
-  simp [valid_judgement.obvious]
-  unfold body
-  repeat unfold substitute
-  simp
-
--- (K (ty_k) (ty_k) k k) : ty_k
-example : valid_judgement ctx (call (call (call (call k ty_k) ty_k) k) k) ty_k := by
-  apply (valid_judgement.call ctx
-    ((((k.call ty_k).call ty_k).call k).call k)
-    ty_k
-    (((k.call ty_k).call ty_k).call k)
-    k
-    (var 1) -- This might be wrong
-    ty_k
-    (by simp))
-  apply (valid_judgement.call ctx
-    (((k.call ty_k).call ty_k).call k)
-    (var 1)
-    ((k.call ty_k).call ty_k)
-    k
-    (ty_k ~> ty_k ~> ty_k)
-    ty_k
-    (by simp))
-  apply (valid_judgement.call ctx
-    ((k.call ty_k).call ty_k)
-    (ty_k ~> ty_k ~> ty_k)
-    (k.call ty_k)
-    ty_k
-    ((var 1) ~> ty_k ~> (var 3) ~> ty_k)
-    (var 1)
-    (by simp)
-  )
-  apply (valid_judgement.call ctx
-    (k.call ty_k)
-    ((var 1) ~> ty_k ~> (var 3) ~> ty_k)
-    k
-    ty_k
-    ty_k
-    (var 1)
-    (by simp)
-  )
-  simp [valid_judgement.k]
-  unfold ty_k
-  apply (valid_judgement.fall ctx
-    (var 1 ~> var 1 ~> var 3 ~> var 3 ~> var 4)
-    (var 1)
-    (var 1)
-    (var 1 ~> var 3 ~> var 3 ~> var 4)
-    (var 1)
-    (by simp)
-  )
-  apply (valid_judgement.fall (var 1 :: ctx)
-    (var 1 ~> var 3 ~> var 3 ~> var 4)
-    (var 1)
-    
-  )
-
-
-
-#eval2
-  sorry
-
